proof-libs/fstar/rust_primitives/Rust_primitives.Hax.Int.fst
@@ -2,7 +2,6 @@ module Rust_primitives.Hax.Int
 
 open Core
 open Rust_primitives
-module LI = Lib.IntTypes
 
 unfold let from_machine (#t:inttype) (x:int_t t) : range_t t = v #t x
 unfold let into_machine (#t:inttype) (n:range_t t) : int_t t = mk_int #t n
